1) fixed all the admits about simulation relations. Our extended memory simulation relations are not bijective mapping between source and target programs, the interesting case is that undef values are mapped to anything, (other kinds of values are mapped exactly w.r.t a mapping function), so this means if a source program uses an undefined value as a conditional value for jmps, the target program can jmp to other locations.
The root problem is that our semantics is determinastic, and takes a
fixed value for undef, say 0. The non-det version of the semantics
should not have the issue, since no matter where the target program
jumps to, it is a valid state included by its source program.

With the det-opsem, we proved that if undefined values are not used for
jmp conditions, size of memory allocations, indices of GEP, the target program 
preserves its original program's state.

2) The rest admitted lemmas are all about freshness --- SBpass correctly
inserts fresh variables.



git-svn-id: https://webdav.seas.upenn.edu/svn/sol/vol@3021 eef5ea85-cc2e-0410-bd84-0fae1f012da8

src/SoftBound/sb_ds_sim.v
@@ -620,6 +620,198 @@ match (ogvs, cs) with
 end.
 
 
+Fixpoint incomingValues_simulation (mi:Values.meminj)
+  (re1:list (id * GenericValue * monad metadata))(rm2:rmap)
+  (re2:list (id * GenericValue)) : Prop :=
+match (re1, re2) with
+| (nil, nil) => True
+| ((i1,gv1,None)::re1', (i2,gv2)::re2') =>
+    i1 = i2 /\ gv_inject mi gv1 gv2 /\ incomingValues_simulation mi re1' rm2 re2'
+| ((i1,gv1,Some (SBopsem.mkMD bgv1 egv1))::re1', 
+   (eid2,egv2)::(bid2,bgv2)::(i2,gv2)::re2') =>
+    i1 = i2 /\ gv_inject mi gv1 gv2 /\ 
+    lookupAL _ rm2 i2 = Some (bid2,eid2) /\
+    gv_inject mi bgv1 bgv2 /\ gv_inject mi egv1 egv2 /\
+    incomingValues_simulation mi re1' rm2 re2'
+| _ => False
+end.
+
+Definition defined_gv (gv:GenericValue) : Prop :=
+match gv with
+| (v,_)::_ => v <> Vundef
+| _ => True
+end.
+
+Fixpoint defined_gvs (gvs:list GenericValue) : Prop :=
+match gvs with
+| gv::gvs' => defined_gv gv /\ defined_gvs gvs'
+| nil => True
+end.
+
+Definition chunk_matched (gv gv':GenericValue) : Prop :=
+let '(_,ms):=split gv in
+let '(_,ms'):=split gv' in
+ms = ms'.
+
+Definition nondet_state sbSt (St : LLVMopsem.State) : Prop :=
+  match sbSt, St with 
+  | {| CurTargetData := TD;
+       ECS := {| CurCmds := insn_gep id0 inbounds0 t vp idxs :: cs;
+                 Locals := lc |} :: _;
+       Globals := gl |}, _ =>
+      match (values2GVs TD idxs lc gl) with
+      | Some vidxs => ~ defined_gvs vidxs
+      | _ => False
+      end
+  | {| CurTargetData := TD;
+       ECS := {| CurCmds := insn_extractvalue _ _ v _ :: _;
+                 Locals := lc |} :: _;
+       Globals := gl |},
+    {| LLVMopsem.CurTargetData := _;
+       LLVMopsem.ECS := {| LLVMopsem.CurCmds := insn_extractvalue _ _ v' _ :: _;
+                 LLVMopsem.Locals := lc' |} :: _;
+       LLVMopsem.Globals := _ |} =>
+      v = v' /\
+      match (getOperandValue TD v lc gl, getOperandValue TD v' lc' gl) with
+      | (Some gv, Some gv') => ~ chunk_matched gv gv'
+      | _ => False
+      end
+  | {| CurTargetData := TD;
+       ECS := {| CurCmds := insn_insertvalue _ _ v1 _ v2 _ :: _;
+                 Locals := lc |} :: _;
+       Globals := gl |},
+    {| LLVMopsem.CurTargetData := _;
+       LLVMopsem.ECS := 
+              {| LLVMopsem.CurCmds := insn_insertvalue _ _ v1' _ v2' _ :: _;
+                 LLVMopsem.Locals := lc' |} :: _;
+       LLVMopsem.Globals := _ |} =>
+      v1 = v1' /\ v2 = v2' /\
+      match (getOperandValue TD v1 lc gl, getOperandValue TD v1' lc' gl,
+             getOperandValue TD v2 lc gl, getOperandValue TD v2' lc' gl) with
+      | (Some gv1, Some gv1', Some gv2, Some gv2') => 
+          ~ chunk_matched gv1 gv1' \/  ~ chunk_matched gv2 gv2'
+      | _ => False
+      end
+  | {| CurTargetData := TD;
+       ECS := {| CurCmds := insn_select id0 v0 _ _ _ :: cs;
+                 Locals := lc |} :: _;
+       Globals := gl |}, _ =>
+      match (getOperandValue TD v0 lc gl) with
+      | Some gv => ~ defined_gv gv
+      | _ => False
+      end
+  | {| CurTargetData := TD;
+       ECS := {| CurCmds := insn_malloc _ _ v0 _ :: cs;
+                 Locals := lc |} :: _;
+       Globals := gl |}, _
+  | {| CurTargetData := TD;
+       ECS := {| CurCmds := insn_alloca _ _ v0 _ :: cs;
+                 Locals := lc |} :: _;
+       Globals := gl |}, _ =>
+      match (getOperandValue TD v0 lc gl) with
+      | Some gv => ~ defined_gv gv
+      | _ => False
+      end
+  | {| CurTargetData := TD;
+       ECS := {| CurCmds := nil; Terminator := insn_br _ Cond _ _;
+                 Locals := lc |} :: _;
+       Globals := gl |}, _ =>
+      match (getOperandValue TD Cond lc gl) with
+      | Some gv => ~ defined_gv gv
+      | _ => False
+      end
+  | _, _ => False
+  end.
+
+Ltac destruct_ctx_br :=
+match goal with
+| [Hsim : sbState_simulates_State _ _
+           {|
+           SBopsem.CurSystem := _;
+           SBopsem.CurTargetData := ?TD;
+           SBopsem.CurProducts := _;
+           SBopsem.ECS := {|
+                          SBopsem.CurFunction := ?F;
+                          SBopsem.CurBB := _;
+                          SBopsem.CurCmds := nil;
+                          SBopsem.Terminator := _;
+                          SBopsem.Locals := _;
+                          SBopsem.Rmap := _;
+                          SBopsem.Allocas := _ |} :: _;
+           SBopsem.Globals := _;
+           SBopsem.FunTable := _;
+           SBopsem.Mem := _;
+           SBopsem.Mmap := _ |} ?St |- _] =>
+  destruct St as [S2 TD2 Ps2 ECs2 gl2 fs2 M2];
+  destruct TD as [los nts];
+  destruct Hsim as [Hwfs [HMinS [Htsym [Heq1 [Htps [HsimECs [Htprds [Hfsim [Hwfg 
+    [Hwfmi HsimM]]]]]]]]]];
+    subst;
+  destruct ECs2 as [|[F2 B2 cs2 tmn2 lc2 als2] ECs2];
+    try solve [inversion HsimECs];
+  simpl in HsimECs;
+  destruct HsimECs as [HsimEC HsimECs];
+  destruct F as [fh1 bs1];
+  destruct F2 as [fh2 bs2];
+  destruct HsimEC as [Hclib [HBinF [HFinPs [Htfdef [Heq0 [Hasim [Hnth [Heqb1 
+    [Heqb2 [ex_ids [rm2 [ex_ids3 [ex_ids4 [cs22 [cs23 [Hgenmeta [Hrsim [Hinc 
+    [Hfresh [Htcmds [Httmn Heq2]]]]]]]]]]]]]]]]]]]]]; subst
+end.
+
+Ltac destruct_ctx_return :=
+match goal with
+| [Hsim : sbState_simulates_State _ _
+           {|
+           SBopsem.CurSystem := _;
+           SBopsem.CurTargetData := ?TD;
+           SBopsem.CurProducts := _;
+           SBopsem.ECS := {|
+                          SBopsem.CurFunction := ?F;
+                          SBopsem.CurBB := _;
+                          SBopsem.CurCmds := nil;
+                          SBopsem.Terminator := _;
+                          SBopsem.Locals := _;
+                          SBopsem.Rmap := _;
+                          SBopsem.Allocas := _ |}
+                          :: {|
+                             SBopsem.CurFunction := ?F';
+                             SBopsem.CurBB := _;
+                             SBopsem.CurCmds := ?c' :: _;
+                             SBopsem.Terminator := _;
+                             SBopsem.Locals := _;
+                             SBopsem.Rmap := _;
+                             SBopsem.Allocas := _ |} :: _;
+           SBopsem.Globals := _;
+           SBopsem.FunTable := _;
+           SBopsem.Mem := _;
+           SBopsem.Mmap := _ |} ?St |- _] =>
+  destruct St as [S2 TD2 Ps2 ECs2 gl2 fs2 M2];
+  destruct TD as [los nts];
+  destruct Hsim as [Hwfs [HMinS [Htsym [Heq1 [Htps [HsimECs [Htprds [Hfsim [Hwfg 
+    [Hwfmi HsimM]]]]]]]]]];
+    subst;
+  destruct ECs2 as [|[F2 B2 cs2 tmn2 lc2 als2] ECs2];
+    try solve [inversion HsimECs];
+  simpl in HsimECs;
+  destruct HsimECs as [HsimEC HsimECs];
+  destruct ECs2 as [|[F2' B2' cs2' tmn2' lc2' als2'] ECs2];
+    try solve [inversion HsimECs];
+  destruct HsimECs as [HsimEC' HsimECs];
+  destruct F as [fh1 bs1];
+  destruct F2 as [fh2 bs2];
+  destruct HsimEC as [Hclib [HBinF [HFinPs [Htfdef [Heq0 [Hasim [Hnth [Heqb1 
+    [Heqb2 [ex_ids [rm2 [ex_ids3 [ex_ids4 [cs22 [cs23 [Hgenmeta [Hrsim [Hinc 
+    [Hfresh [Htcmds [Httmn Heq2]]]]]]]]]]]]]]]]]]]]]; subst;
+  destruct F' as [fh1' bs1'];
+  destruct F2' as [fh2' bs2'];
+  destruct c'; try solve [inversion HsimEC'];
+  destruct HsimEC' as [Hclib' [HBinF' [HFinPs' [Htfdef' [Heq0' [Hasim' [Hnth' 
+    [Heqb1' [Heqb2' [ex_ids' [rm2' [ex_ids3' [ex_ids4' [cs22' [cs23' [cs24' 
+    [Hgenmeta' [Hrsim' [Hinc' [Hcall' [Hfresh' [Htcmds' [Httmn' Heq2']]]]]]]]]]]]
+    ]]]]]]]]]]]; 
+    subst
+end.
+
 (*****************************)
 (*
 *** Local Variables: ***
